clight2rustlight/Clight2Rustlight.v
@@ -28,7 +28,64 @@ Require Import rustfrontend.Rustlight.
 
 Import ListNotations.
 
-Local Open Scope error_monad_scope.
+(* Local Open Scope error_monad_scope. *)
+
+Parameter dummy_origin : unit -> origin.
+
+(** State and error monad for generating fresh identifiers. *)
+
+Record generator : Type := mkgenerator {
+  gen_next: ident;
+  gen_trail: list (ident * type)
+}.
+
+Inductive result (A: Type) (g: generator) : Type :=
+  | Err: Errors.errmsg -> result A g
+  | Res: A -> forall (g': generator), Ple (gen_next g) (gen_next g') -> result A g.
+
+Arguments Err [A g].
+Arguments Res [A g].
+
+Definition mon (A: Type) := forall (g: generator), result A g.
+
+Definition ret {A: Type} (x: A) : mon A :=
+  fun g => Res x g (Ple_refl (gen_next g)).
+
+Definition error {A: Type} (msg: Errors.errmsg) : mon A :=
+  fun g => Err msg.
+
+Definition bind {A B: Type} (x: mon A) (f: A -> mon B) : mon B :=
+  fun g =>
+    match x g with
+      | Err msg => Err msg
+      | Res a g' i =>
+          match f a g' with
+          | Err msg => Err msg
+          | Res b g'' i' => Res b g'' (Ple_trans _ _ _ i i')
+      end
+    end.
+
+Definition bind2 {A B C: Type} (x: mon (A * B)) (f: A -> B -> mon C) : mon C :=
+  bind x (fun p => f (fst p) (snd p)).
+
+Declare Scope gensym_monad_scope.
+Notation "'do' X <- A ; B" := (bind A (fun X => B))
+   (at level 200, X ident, A at level 100, B at level 200)
+   : gensym_monad_scope.
+Notation "'do' ( X , Y ) <- A ; B" := (bind2 A (fun X Y => B))
+   (at level 200, X ident, Y ident, A at level 100, B at level 200)
+   : gensym_monad_scope.
+
+Parameter first_unused_ident: unit -> ident.
+
+Definition initial_generator (x: unit) : generator :=
+  mkgenerator (first_unused_ident x) nil.
+
+Definition gensym (ty: type): mon ident :=
+  fun (g: generator) =>
+    Res (gen_next g)
+        (mkgenerator (Pos.succ (gen_next g)) ((gen_next g, ty) :: gen_trail g))
+        (Ple_succ (gen_next g)).
 
 (** Convert Clight type to Rustlight type *)
 Fixpoint to_rusttype (ty: Ctypes.type): Rusttypes.type :=
@@ -39,10 +96,9 @@ Fixpoint to_rusttype (ty: Ctypes.type): Rusttypes.type :=
   | Ctypes.Tfloat fz _ => Rusttypes.Tfloat fz
   | Ctypes.Tstruct id _ => Rusttypes.Tstruct nil id
   | Ctypes.Tunion id _ => Rusttypes.Tvariant nil id
-  (* FIXME: 1%positive *)
-  | Ctypes.Tpointer ty _ => Rusttypes.Treference 1%positive Mutable (to_rusttype ty)
+  | Ctypes.Tpointer ty _ => Rusttypes.Traw_pointer mutable (to_rusttype ty)
   (*todo*)
-  | Ctypes.Tarray ty' sz _ => Rusttypes.Tarray (to_rusttype ty') sz
+  | Ctypes.Tarray ty' sz _ => Rusttypes.Tarray Mutable (to_rusttype ty') sz
   | Ctypes.Tfunction tyl ty' cc => 
       Rusttypes.Tfunction nil nil (to_rustlight tyl) (to_rusttype ty') cc
   end
@@ -80,68 +136,83 @@ End MEMORY.
     Variable tce: Rusttypes.composite_env.
 
     Local Open Scope string_scope.
-
-    Local Open Scope error_monad_scope.
+    Local Open Scope gensym_monad_scope.
     
 
     (** Convert Clight expression to Rustlight place *)
-    Fixpoint cexpr_to_place (e: Clight.expr): res Rustlight.place :=
+    Fixpoint cexpr_to_place (e: Clight.expr): mon Rustlight.place :=
       match e with
-      | Clight.Evar id ty =>OK (Rustlight.Plocal id (to_rusttype ty))
+      | Clight.Evar id ty => ret (Rustlight.Plocal id (to_rusttype ty))
+      | Clight.Etempvar id ty => ret (Rustlight.Plocal id (to_rusttype ty))
       | Clight.Ederef e' ty=>
           do p <- cexpr_to_place e';
-          OK (Rustlight.Pderef p (to_rusttype ty))
+          ret (Rustlight.Pderef p (to_rusttype ty))
       | Clight.Efield e' id ty => 
           do p <- cexpr_to_place e';
-          OK (Rustlight.Pfield p id (to_rusttype ty))
+          ret (Rustlight.Pfield p id (to_rusttype ty))
+      | Clight.Ebinop op e1 e2 ty => 
+          match ty with
+          | Ctypes.Tpointer _ _ =>
+              do i <- gensym (to_rusttype ty);
+              ret (Rustlight.Pparenthesize i (to_rusttype ty))
+          | _ =>
+              error (msg "not pointer, Unsupported lvalue expression")
+          end
       (* FIXME: support Pdowncast *)
-      | _ => Error (msg "Unsupported lvalue expression")
+      | _ => error (msg "Unsupported lvalue expression")
       end.
 
     (** Convert Clight expression to Rustlight pure expression *)
-    Fixpoint cexpr_to_pexpr (locals: list ident) (e: Clight.expr): res Rustlight.pexpr :=
+    Fixpoint cexpr_to_pexpr (locals: list ident) (e: Clight.expr): mon Rustlight.pexpr :=
       match e with
-      | Clight.Econst_int i ty => OK (Rustlight.Econst_int i (to_rusttype ty))
-      | Clight.Econst_float f ty => OK (Rustlight.Econst_float f (to_rusttype ty))
-      | Clight.Econst_single f ty => OK (Rustlight.Econst_single f (to_rusttype ty))
-      | Clight.Econst_long l ty => OK (Rustlight.Econst_long l (to_rusttype ty))
+      | Clight.Econst_int i ty => ret (Rustlight.Econst_int i (to_rusttype ty))
+      | Clight.Econst_float f ty => ret (Rustlight.Econst_float f (to_rusttype ty))
+      | Clight.Econst_single f ty => ret (Rustlight.Econst_single f (to_rusttype ty))
+      | Clight.Econst_long l ty => ret (Rustlight.Econst_long l (to_rusttype ty))
       | Clight.Eunop op e' ty => 
           do pe <- cexpr_to_pexpr locals e';
-          OK (Rustlight.Eunop op pe (to_rusttype ty))
+          ret (Rustlight.Eunop op pe (to_rusttype ty))
       | Clight.Ebinop op e1 e2 ty => 
           do pe1 <- cexpr_to_pexpr locals e1;
           do pe2 <- cexpr_to_pexpr locals e2;
-          OK (Rustlight.Ebinop op pe1 pe2 (to_rusttype ty))
+          ret (Rustlight.Ebinop op pe1 pe2 (to_rusttype ty))
       | Clight.Evar id ty => 
           if in_dec ident_eq id locals then
             do p <- cexpr_to_place (Clight.Evar id ty);
-            OK (Eplace p (to_rusttype ty))
+            ret (Eplace p (to_rusttype ty))
           else
-            OK (Eglobal id (to_rusttype ty))
+            ret (Eglobal id (to_rusttype ty))
+      | Clight.Etempvar id ty =>
+        (* if in_dec ident_eq id locals then
+          do p <- cexpr_to_place (Clight.Evar id ty);
+          ret (Eplace p (to_rusttype ty))
+        else *)
+          do p <- cexpr_to_place (Clight.Evar id ty);
+          ret (Eplace p (to_rusttype ty))
       | Clight.Eaddrof e ty => 
           do p <- cexpr_to_place e;
-          OK (Eref 2%positive Mutable p (to_rusttype ty))
+          ret (Eref 2%positive Mutable p (to_rusttype ty))
       | Clight.Ederef e ty => 
           do p <- cexpr_to_place e;
-          OK (Rustlight.Eplace (Rustlight.Pderef p (to_rusttype ty)) (to_rusttype ty))
+          ret (Rustlight.Eplace (Rustlight.Pderef p (to_rusttype ty)) (to_rusttype ty))
       | Clight.Efield e' id ty => 
           do p <- cexpr_to_place e';
-          OK (Rustlight.Eplace (Rustlight.Pfield p id (to_rusttype ty)) (to_rusttype ty))
+          ret (Rustlight.Eplace (Rustlight.Pfield p id (to_rusttype ty)) (to_rusttype ty))
       (* | Clight.Ecast e' ty => cexpr_to_pexpr locals e'
-      | Clight.Esizeof ty ty' => OK (Rustlight.Esizeof (to_rusttype ty) (to_rusttype ty')) *)
-      (* | Clight.Ealignof ty ty' => OK (Rustlight.Ealignof (to_rusttype ty) (to_rusttype ty')) *)
+      | Clight.Esizeof ty ty' => ret (Rustlight.Esizeof (to_rusttype ty) (to_rusttype ty')) *)
+      (* | Clight.Ealignof ty ty' => ret (Rustlight.Ealignof (to_rusttype ty) (to_rusttype ty')) *)
       (*FIXME ???*)
       (*  *)
-      | _ => Error (msg "Unsupported rvalue expression")
+      | _ => error (msg "Unsupported rvalue expression")
       end.
 
-    Fixpoint transl_expr_list (locals: list ident) (el: list Clight.expr) : res (list Rustlight.pexpr) :=
+    Fixpoint transl_expr_list (locals: list ident) (el: list Clight.expr) : mon (list Rustlight.pexpr) :=
       match el with
-      | nil => OK nil
+      | nil => ret nil
       | e :: rest =>
           do pe <- cexpr_to_pexpr locals e;
           do rest' <- transl_expr_list locals rest;
-          OK (pe :: rest')
+          ret (pe :: rest')
       end.
 
     Definition pexpr_to_expr (pe: Rustlight.pexpr): Rustlight.expr :=
@@ -151,32 +222,32 @@ End MEMORY.
       Rustlight.Plocal 1%positive Rusttypes.Tunit. 
     
 
-    Fixpoint transl_stmt (locals: list ident) (s: Clight.statement): res Rustlight.statement :=
+    Fixpoint transl_stmt (locals: list ident) (s: Clight.statement): mon Rustlight.statement :=
       let transl_stmt := transl_stmt locals in
       match s with
-      | Clight.Sskip => OK Rustlight.Sskip
+      | Clight.Sskip => ret Rustlight.Sskip
       | Clight.Ssequence s1 s2 => 
           do rs1 <- transl_stmt s1;
           do rs2 <- transl_stmt s2;
-          OK (Rustlight.Ssequence rs1 rs2)
+          ret (Rustlight.Ssequence rs1 rs2)
       | Clight.Sifthenelse e s1 s2 => 
           do pe <- cexpr_to_pexpr locals e;
           do rs1 <- transl_stmt s1;
           do rs2 <- transl_stmt s2;
-          OK (Rustlight.Sifthenelse (Rustlight.Epure pe) rs1 rs2)
+          ret (Rustlight.Sifthenelse (Rustlight.Epure pe) rs1 rs2)
       | Clight.Sloop s1 s2 => 
           do rs1 <- transl_stmt s1;
-          OK (Rustlight.Sloop rs1)
-      | Clight.Sbreak => OK Rustlight.Sbreak
-      | Clight.Scontinue => OK Rustlight.Scontinue
+          ret (Rustlight.Sloop rs1)
+      | Clight.Sbreak => ret Rustlight.Sbreak
+      | Clight.Scontinue => ret Rustlight.Scontinue
       | Clight.Sassign e1 e2 => 
           do p <- cexpr_to_place e1;
           do pe <- cexpr_to_pexpr locals e2;
-          OK (Rustlight.Sassign p (Rustlight.Epure pe))
-      (* | Clight.Sset id e => 
+          ret (Rustlight.Sassign p (Rustlight.Epure pe))
+      | Clight.Sset id e => 
           do pe <- cexpr_to_pexpr locals e;
-          OK (Rustlight.Sassign (Rustlight.Plocal id (to_rusttype (Clight.typeof e))) 
-                (Rustlight.Epure pe)) *)
+          ret (Rustlight.Sassign (Rustlight.Plocal id (to_rusttype (Clight.typeof e))) 
+                (Rustlight.Epure pe))
       | Clight.Scall optid e args =>
           do pe <- cexpr_to_pexpr locals e;
           do pargs <- transl_expr_list locals args;
@@ -184,58 +255,65 @@ End MEMORY.
           | None => 
               (* without return value *)
               let dummy_place := empty_place in
-              OK (Rustlight.Scall dummy_place (Rustlight.Epure pe) (map pexpr_to_expr pargs))
+              ret (Rustlight.Scall dummy_place (Rustlight.Epure pe) (map pexpr_to_expr pargs))
           | Some id => 
               (* with return value *)
               let ret_ty := to_rusttype (Clight.typeof e) in
               let place := Rustlight.Plocal id ret_ty in
-              OK (Rustlight.Scall place (Rustlight.Epure pe) (map pexpr_to_expr pargs))
+              ret (Rustlight.Scall place (Rustlight.Epure pe) (map pexpr_to_expr pargs))
           end
       | Clight.Sreturn None => 
           (* no return value*)
-          OK (Rustlight.Sreturn empty_place)
+          ret (Rustlight.Sreturn empty_place)
       | Clight.Sreturn (Some e) => 
           do pe <- cexpr_to_pexpr locals e;
           (* create a temp variable to store return value *)
           let ret_place := Rustlight.Plocal 2%positive (to_rusttype (Clight.typeof e)) in
           (* assign the return value to the temp variable and return *)
-          OK (Rustlight.Ssequence
+          ret (Rustlight.Ssequence
                 (Rustlight.Sassign ret_place (Rustlight.Epure pe))
                 (Rustlight.Sreturn ret_place))
       (* | Clight.Sswitch e cases =>
         do pe <- cexpr_to_pexpr locals e;
-        let fix convert_cases (cases: Clight.labeled_statements) : res Rustlight.statement :=
+        let fix convert_cases (cases: Clight.labeled_statements) : mon Rustlight.statement :=
             match cases with
-            | nil => OK Rustlight.Sskip
+            | nil => ret Rustlight.Sskip
             | Clight.LScase n s rest =>
                 do rs <- transl_stmt s;
                 do rest_stmt <- convert_cases rest;
                 let cond := Rustlight.Ebinop Ceq (Rustlight.Epure pe) 
                                              (Rustlight.Econst_int n (to_rusttype (Clight.typeof e))) 
                                              Rusttypes.Tbool in
-                OK (Rustlight.Sifthenelse cond rs rest_stmt)
+                ret (Rustlight.Sifthenelse cond rs rest_stmt)
             | Clight.LSdefault s rest =>
                 transl_stmt s
             end
         in
         convert_cases cases *)
-      | _ => Error (msg "Unsupported statement type")
+      | _ => error (msg "Unsupported statement type")
       end.
 
     (** Convert Clight function to Rustlight function *)
     Definition transl_function (f: Clight.function): res Rustlight.function :=
       let locals := List.map (@fst ident _) (Clight.fn_params f ++ Clight.fn_vars f) in
-      do body <- transl_stmt locals (Clight.fn_body f);
+      match transl_stmt locals (Clight.fn_body f) (initial_generator tt) with
+      | Err msg =>
+          Error msg
+      | Res body g i =>
       OK {| Rustlight.fn_generic_origins := [];
            Rustlight.fn_origins_relation := [];
            Rustlight.fn_drop_glue := None;
            Rustlight.fn_return := to_rusttype (Clight.fn_return f);
            Rustlight.fn_callconv := (Clight.fn_callconv f);
            (* save temp variable in clight in stack(fn_vars) *)
-           Rustlight.fn_vars := List.map (fun '(id, ty) => (id, to_rusttype ty)) (Clight.fn_vars f ++ Clight.fn_temps f);
+           (* FIXME *)
+           Rustlight.fn_vars := (List.map (fun '(id, ty) => (id, to_rusttype ty)) (Clight.fn_vars f ++ Clight.fn_temps f)) ++ g.(gen_trail);
            Rustlight.fn_params := List.map (fun '(id, ty) => (id, to_rusttype ty)) (Clight.fn_params f);
            Rustlight.fn_body := body
-         |}.
+         |}
+        end.
+
+         Local Open Scope error_monad_scope.
 
     Definition transl_fundef (id: ident) (f: Clight.fundef): res Rustlight.fundef :=
       match f with
@@ -257,8 +335,8 @@ End MEMORY.
           match f with
           | Internal fd =>
               Gfun (Internal fd)
-          | External origins org_rels ef args res cc =>
-              Gfun (External origins org_rels ef args res cc) 
+          | External origins org_rels ef args mon cc =>
+              Gfun (External origins org_rels ef args mon cc) 
           end
       | Gvar v =>
           Gvar {|
@@ -269,21 +347,23 @@ End MEMORY.
             |}
       end.
 
-    Fixpoint convert_members (ms:Ctypes.members) : res Rusttypes.members :=
+      Local Open Scope gensym_monad_scope.
+
+    Fixpoint convert_members (ms:Ctypes.members) : mon Rusttypes.members :=
       match ms with
-      | nil => OK (nil)
+      | nil => ret (nil)
       | h::t => match h with
                 | (Ctypes.Member_plain id ty) =>
                     do cm <- convert_members t;
-                    OK ((Rusttypes.Member_plain id (to_rusttype ty)) :: cm)
+                    ret ((Rusttypes.Member_plain id (to_rusttype ty)) :: cm)
                 | (Ctypes.Member_bitfield id _ _ _ _ _) =>
-                    Error (msg "not support member bitfield")
+                    error (msg "not support member bitfield")
                 end
       end.
 
-    Fixpoint convert_composite_definition (cd:list Ctypes.composite_definition) : res (list Rusttypes.composite_definition) :=
+    Fixpoint convert_composite_definition (cd:list Ctypes.composite_definition) : mon (list Rusttypes.composite_definition) :=
       match cd with
-      | nil => OK (nil)
+      | nil => ret (nil)
       | (Ctypes.Composite id su m a)::t =>
           let new_su := match su with
                         | Ctypes.Struct => Rusttypes.Struct
@@ -291,27 +371,32 @@ End MEMORY.
                         end in
           do new_m <- convert_members m;
           do rcd <- convert_composite_definition t;
-          OK ((Rusttypes.Composite id new_su new_m [] []) :: rcd)
+          ret ((Rusttypes.Composite id new_su new_m [] []) :: rcd)
       end.
 
+Local Open Scope error_monad_scope.
+
     Definition transl_program (p: Clight.program): res program :=
-      match convert_composite_definition (Ctypes.prog_types p) with
-      | OK co_defs =>
+      let initial_gen := initial_generator tt in
+      match convert_composite_definition (Ctypes.prog_types p) initial_gen with
+      | Res co_defs g i =>
           let tce := Rusttypes.build_composite_env co_defs in
-          (match tce as m return (tce = m) -> res program with
-           | OK tce =>
-               fun Hyp =>
-                 let ce := Ctypes.prog_comp_env p in
-                 do p1 <- transform_partial_program2 transl_fundef transl_globvar p;
-                 OK {| Rusttypes.prog_defs := AST.prog_defs p1;
-                      Rusttypes.prog_public := AST.prog_public p1;
-                      Rusttypes.prog_main := AST.prog_main p1;
-                      Rusttypes.prog_types := co_defs;
-                      Rusttypes.prog_comp_env := tce;
-                      Rusttypes.prog_comp_env_eq := Hyp |}
-           | Error msg => fun _ => Error msg
-           end) (eq_refl tce)
-      | _ =>Error (msg "error in transl_composites (clight2rustlight)")
-      end.
+          (match tce with
+          | OK tce =>
+          fun Hyp =>
+              let ce := Ctypes.prog_comp_env p in
+              do p1 <- transform_partial_program2 transl_fundef transl_globvar p;
+              OK {| Rusttypes.prog_defs := AST.prog_defs p1;
+                    Rusttypes.prog_public := AST.prog_public p1;
+                    Rusttypes.prog_main := AST.prog_main p1;
+                    Rusttypes.prog_types := co_defs;
+                    Rusttypes.prog_comp_env := tce;
+                    Rusttypes.prog_comp_env_eq := Hyp |}
+                    | Error msg => fun _ => Error msg
+                    end) (eq_refl tce)
+          | Err msg => Error msg
+          end.
+      (* | Err msg => Error msg
+      end. *)
   
     End TRANSL.
