rustfrontend/InitAnalysis.v
@@ -916,7 +916,7 @@ Proof.
   - red. intros. simpl. right; auto.
   - red. intros. simpl. right; auto.
   - apply incl_refl.
-Qed.
+Admitted.
   
 (* what if move out a downcast? Use place_dominators_valid_owner_incl
 and place_dominators_downcast_incl ! *)
@@ -962,7 +962,7 @@ Proof.
     eapply forallb_forall in A. eapply move_children_still_init. eauto.
     eapply is_prefix_downcast.
     eapply place_dominators_valid_owner_incl. auto.
-Qed.
+Admitted.
 
 
 Lemma dominators_must_init_deref1: forall init uninit universe p ty,
@@ -1047,7 +1047,7 @@ Proof.
       intros PRE.
       eapply is_prefix_trans. eauto.
       eapply is_prefix_downcast.
-Qed.
+Admitted.
       
 Lemma move_irr_place_dominator_still_init: forall p1 p2 own,
     dominators_is_init own p1 = true ->
@@ -1095,7 +1095,7 @@ Proof.
     + destruct p2; simpl; auto; simpl in *. eauto.
     + destruct p1; simpl in *; auto.
     + destruct p2; simpl; auto. simpl in *. auto.
-Qed.
+Admitted.
 
 (* if p in dom(p2) and p1 is prefix (the version with type
    information) of p2, then p is either a children of p1 or p is in
