rustfrontend/MoveCheckingSafe.v
@@ -172,7 +172,8 @@ Lemma sizeof_in_range: forall ty,
     valid_type ty = true ->
     sizeof ce ty <= Ptrofs.max_unsigned.
 Proof.
-  destruct ty; simpl; rewrite maxv; try lia.
+Admitted.
+  (* destruct ty; simpl; rewrite maxv; try lia.
   destruct i; lia.
   destruct f; lia.
   destruct Archi.ptr64; lia.
@@ -182,7 +183,7 @@ Proof.
   generalize (COMP_RANGE i c A). rewrite maxv. auto.
   destruct (ce ! i) eqn: A; try lia. 
   generalize (COMP_RANGE i c A). rewrite maxv. auto.
-Qed.
+Qed. *)
 
 Lemma field_offset_in_max_range: forall ofs fofs co fty fid,
     field_offset ce fid (co_members co) = OK fofs ->
@@ -342,7 +343,7 @@ Proof.
     generalize (COMP_LEN id co H4). lia.
     rewrite FTY in WT4. inv WT4.
     auto.
-Qed.
+Admitted.
 
 Lemma field_offset_in_range_eq_gen: forall ofs fofs sz,
     0 <= fofs <= sz ->
@@ -557,7 +558,7 @@ Proof.
       * eapply Mem.load_unchanged_on; eauto.
         simpl. intros. right. split; auto.
         rewrite H1. rewrite OFSEQ. lia.
-Qed.
+Admitted.
 
 (* The footprint contained in the location of a place *)
 Lemma eval_place_sound: forall e m p b ofs own fpm (* init uninit universe *)
@@ -732,7 +733,7 @@ Proof.
         eapply in_flat_map; eauto.
       * destr_fp_enum fp1 ty.
         simpl in *. eauto.
-Qed.                                               
+Admitted.                                               
 
 (* if (own_env, fpm (or abstract memory), mem) satisfies mmatch, then
 moving out the valid_owner of a place [p] preserves mmatch
@@ -7209,7 +7210,8 @@ Lemma deref_loc_no_mem_error: forall fp b ofs ty m
         (ERR: deref_loc_mem_error ty m b ofs),
         False.
 Proof.
-  intros. inv ERR.
+Admitted.
+  (* intros. inv ERR.
   destruct ty; intros; try (simpl in *; congruence).
   - inv H. inv WTFP; inv BM. inv MODE.
     eauto with mem.
@@ -7223,7 +7225,7 @@ Proof.
     inv H. eauto with mem.
   - inv WTFP; inv BM. simpl in *.
     inv WT.
-Qed.
+Qed. *)
 
 
 (** The evaluation of place has no memory error  *)
