rustfrontend/RustOp.v
@@ -438,20 +438,20 @@ Proof.
   - destruct t2; inv H0; simpl in *;
     try(destruct i; destruct (Archi.ptr64));
     try (destruct f0); TrivialInject. 
-  (* - destruct t2; inv H0; simpl in *;
+  - destruct t2; inv H0; simpl in *;
     try(destruct i; destruct (Archi.ptr64)); 
     try (destruct f0); 
     try (destruct (ident_eq i i0~1); TrivialInject); 
     try (destruct (ident_eq i i0~0); TrivialInject); 
     try (inv H);
     try (eapply Val.inject_ptr; eauto). 
-    exists (Vptr b2 (Ptrofs.add ofs1 (Ptrofs.repr delta))).
-    destruct (ident_eq i 1). split. auto.  
-    TrivialInject. eapply Val.inject_ptr; eauto. inv H2. 
+  - destruct t2; inv H0; simpl in *;
+    try(destruct i; destruct (Archi.ptr64)); 
+    try (destruct f0); 
+    try (destruct (ident_eq i i0~1); TrivialInject); 
+    try (destruct (ident_eq i i0~0); TrivialInject); 
+    try (inv H);
     try (eapply Val.inject_ptr; eauto). 
-    exists (Vptr b2 (Ptrofs.add ofs1 (Ptrofs.repr delta))).
-    destruct (ident_eq i 1). split. auto.  
-    TrivialInject. eapply Val.inject_ptr; eauto. inv H2.  *)
   - destruct t2; inv H0; simpl in *;
     try(destruct i0; destruct (Archi.ptr64)); 
     try (destruct f0); 
